Add string fields axiom and move string pure comparison to string semantics (#598)
I needed some string semantics support for an ongoing proof and I think
a lot of this stuff is going to be necessary fairly often:
1. I added a string fields axiom that uses a pure model that splits on
spaces, tabs etc
Note: this is currently unsound for strings with non-ascii runes, this is called out in comments, a fix will be either extending the axiom to support non-ascii or adding a precondition that the string only contains ascii 
2. I moved the string comparison helpers that were in an etcd proof to
strings.v so they can be used broadly

---------

Co-authored-by: Upamanyu Sharma <upamanyu@mit.edu>

new/golang/defn/string.v
@@ -6,6 +6,43 @@ Section defs.
 Context {ext : ffi_syntax}.
 Context {go_lctx : GoLocalContext} {go_gctx : GoGlobalContext}.
 
+Global Instance w8_lexico : Lexico w8 := (λ x y, uint.Z x < uint.Z y).
+
+Global Instance : TrichotomyT (lexico (A:=w8)).
+Proof.
+  intros x y. destruct (uint.Z x ?= uint.Z y) eqn:Heq.
+  - apply Z.compare_eq in Heq. left. right. word.
+  - left. left. rewrite (Z.compare_lt_iff (uint.Z x) (uint.Z y)) in Heq.
+    rewrite /lexico /= /w8_lexico //.
+  - right. rewrite (Z.compare_gt_iff (uint.Z x) (uint.Z y)) in Heq.
+    rewrite /lexico /= /w8_lexico //.
+Defined. (* for computing bool_decide *)
+
+Global Instance : StrictOrder (lexico (A:=w8)).
+Proof.
+  constructor.
+  - intros x. rewrite /lexico /w8_lexico /complement. intros H. lia.
+  - intros x y z. rewrite /lexico /w8_lexico. lia.
+Qed.
+
+Definition go_string_lt : go_string → go_string → Prop := lexico.
+
+Instance : StrictOrder go_string_lt.
+Proof. apply _. Qed.
+
+Example go_string_ltb_examples :
+  ¬ go_string_lt "" "" ∧
+  go_string_lt "" "a" ∧
+  ¬ go_string_lt "a" "" ∧
+  ¬ go_string_lt "ab" "a" ∧
+  go_string_lt "ab" "b".
+Proof.
+  split_and!; eapply bool_decide_unpack; done.
+Qed.
+
+Definition go_string_le (x y : go_string) : Prop :=
+  x = y ∨ go_string_lt x y.
+
 Class StringSemantics `{!GoSemanticsFunctions} :=
 {
   #[global] package_sem :: strings.Assumptions;
@@ -32,6 +69,18 @@ Class StringSemantics `{!GoSemanticsFunctions} :=
   #[global] convert_string_to_bytes
     `[!from ↓u go.string] `[!to ↓u go.SliceType elem_type] `[!elem_type ↓u go.byte] (v : val) ::
     ⟦Convert from to, v⟧ ⤳[internal] (@! strings.StringToByteSlice v);
+
+  #[global] lt_string (x y : go_string) ::
+    ⟦GoOp GoLt go.string, (#x, #y)⟧ ⤳[under] #(bool_decide (go_string_lt x y));
+
+  #[global] le_string (x y : go_string) ::
+    ⟦GoOp GoLe go.string, (#x, #y)⟧ ⤳[under] #(bool_decide (go_string_le x y));
+
+  #[global] gt_string (x y : go_string) ::
+    ⟦GoOp GoGt go.string, (#x, #y)⟧ ⤳[under] #(bool_decide (go_string_lt y x));
+
+  #[global] ge_string (x y : go_string) ::
+    ⟦GoOp GoGe go.string, (#x, #y)⟧ ⤳[under] #(bool_decide (go_string_le y x));
 }.
 End defs.
 End go.
