new/proof/strings.v
@@ -1,5 +1,4 @@
 From New.proof Require Import proof_prelude.
-From New.proof Require Export std.
 From New.generatedproof Require Export strings.
 From Perennial Require Import base.
 
@@ -31,6 +30,103 @@ Proof.
   iIntros "Hown". wp_auto.
   wp_apply wp_asciiSpace_init.
   iEval (rewrite is_pkg_init_unfold /=). iFrame "∗#". done.
+Qed.
+
+(* Model for Go's unicode.IsSpace for ASCII-range bytes.
+   Based on https://cs.opensource.google/go/go/+/refs/tags/go1.26.1:src/strings/strings.go;l=377 *)
+Definition is_ascii_space (b : w8) : bool :=
+  (word.eqb b (W8 9))  ||    (* \t  (0x09) *)
+  (word.eqb b (W8 10)) ||    (* \n  (0x0A) *)
+  (word.eqb b (W8 11)) ||    (* \v  (0x0B) *)
+  (word.eqb b (W8 12)) ||    (* \f  (0x0C) *)
+  (word.eqb b (W8 13)) ||    (* \r  (0x0D) *)
+  (word.eqb b (W8 32))      (* space (0x20) *)
+.
+
+Fixpoint split_fields_aux (s : go_string) (w : option go_string) : list go_string :=
+  match s with
+  | [] => match w with None => [] | Some w => [w] end
+  | x :: s => if is_ascii_space x then
+              match w with
+              | None => split_fields_aux s None
+              | Some w => w :: split_fields_aux s None
+              end
+            else split_fields_aux s (Some (default [] w ++ [x]))
+  end.
+Definition split_fields (s : go_string) : list go_string := split_fields_aux s None.
+
+(* FIXME: this is wrong (unsound) for strings with non-ascii runes. Simplest
+   solution might be to add a precondition for the string to be all ascii. *)
+Axiom wp_Fields :
+  ∀ `{!strings.Assumptions} (s : go_string),
+  {{{ is_pkg_init strings }}}
+    @! strings.Fields #s
+  {{{ sl,
+      RET #sl;
+      sl ↦* (split_fields s) ∗ own_slice_cap w8 sl (DfracOwn 1) }}}.
+
+(* Test split_fields because it is part of the wp_Fields axiom. *)
+Example split_fields_hello :
+  split_fields "hello"%go = ["hello"%go].
+Proof. vm_compute. reflexivity. Qed.
+
+Example split_fields_leading_spaces :
+  split_fields "   hello world"%go = ["hello"%go; "world"%go].
+Proof. vm_compute. reflexivity. Qed.
+
+Example split_fields_two_words :
+  split_fields "hello world"%go = ["hello"%go; "world"%go].
+Proof. vm_compute. reflexivity. Qed.
+
+Example split_fields_empty :
+  split_fields ""%go = [].
+Proof. vm_compute. reflexivity. Qed.
+
+Definition bs_tab : w8 := W8 9.
+Definition bs_nl  : w8 := W8 10.
+Definition bs_cr  : w8 := W8 13.
+Definition bs_sp  : w8 := W8 32.
+
+Definition hello_world_ws : go_string :=
+  [bs_sp; bs_tab] ++ "hello"%go ++ [bs_nl] ++ "world"%go ++ [bs_cr; bs_sp].
+
+Example split_fields_mixed_ws :
+  split_fields hello_world_ws =
+    ["hello"%go; "world"%go].
+Proof. vm_compute. reflexivity. Qed.
+
+Example split_fields_interp_string_literal :
+  split_fields "  hello\tthere\ngeneral\rkenobi "%go
+  = ["hello"%go; "there"%go; "general"%go; "kenobi"%go].
+Proof. vm_compute. reflexivity. Qed.
+
+(* Unit tests for wp_Fields, exercising the axiom via fields_spec *)
+Example wp_Fields_mixed_ws :
+  {{{ is_pkg_init strings }}}
+    @! strings.Fields #("  hello\tthere\ngeneral\rkenobi "%go)
+  {{{ sl,
+      RET #sl;
+      sl ↦* ["hello"%go; "there"%go; "general"%go; "kenobi"%go] ∗ own_slice_cap w8 sl (DfracOwn 1) }}}.
+Proof.
+  iIntros (Φ) "#Hinit HΦ".
+  wp_apply (wp_Fields).
+  iIntros (sl) "(Hsl & Hcap)".
+  iApply "HΦ". iFrame.
+Qed.
+
+Example wp_Fields_two_words:
+  {{{ is_pkg_init strings }}}
+    @! strings.Fields #"hello world"%go
+  {{{ sl,
+      RET #sl;
+      sl ↦* ["hello"%go; "world"%go] ∗
+      own_slice_cap w8 sl (DfracOwn 1)
+  }}}.
+Proof.
+  iIntros (Φ) "#Hinit HΦ".
+  wp_apply (wp_Fields "hello world"%go).
+  iIntros (sl) "(Hsl & Hcap)".
+  iApply "HΦ". iFrame.
 Qed.
 
 End wps.
